prepare extraction, fails with undefined reference

test.c
@@ -1,0 +1,8 @@
+#include "P1_UInt32.c"
+
+int main() {
+  uint32_t ui = P1_UInt32_main ();
+  printf("r=%ui\n", ui);
+  printf("Hello, world!\n");
+  return 0;
+}
