NTreeC3.fst
@@ -624,3 +624,10 @@ let unpack_tree (#a: Type0) (ptr: t a)
   tree_view_aux_same_size (v_node (get_left n) h2);
   tree_view_aux_same_size (v_node (get_right n) h2);
   return n
+
+let create_leaf (#a: Type0) (_: unit) : Steel (t a)
+  emp (fun ptr -> linked_tree ptr)
+  (requires fun _ -> True)
+  (ensures fun _ ptr h1 -> Trees.Leaf? (v_linked_tree ptr h1))
+  = intro_linked_tree_leaf #a ();
+    null_t #a
