P1_UInt32.fst
@@ -1,7 +1,180 @@
 module P1_UInt32
 
-open NTreeC3
-open P1
+open Steel.Memory
+open Steel.Effect.Atomic
+open Steel.Effect
+open Steel.Reference
+//open NTreeC3
+//open P1
 module U32 = FStar.UInt32
+module I32 = FStar.Int32
+module B = LowStar.Buffer
 
-let append_left = append_left #U32.t
+
+let t = NTreeC3.t
+let linked_tree = NTreeC3.linked_tree
+let get_left = NTreeC3.get_left
+let get_right = NTreeC3.get_right
+let get_size = NTreeC3.get_size
+//let is_null = is_null #U32.t
+//let null_t = null_t #U32.t
+//let null_t = null_t #U32.t
+let null = Steel.Reference.null
+let is_null_t = NTreeC3.is_null_t #U32.t
+let mk_node = NTreeC3.mk_node #U32.t
+let unpack_tree = NTreeC3.unpack_tree #U32.t
+
+//inline_for_extraction
+let intro_linked_tree_leaf = NTreeC3.intro_linked_tree_leaf #U32.t
+
+let elim_linked_tree_leaf = NTreeC3.elim_linked_tree_leaf #U32.t
+let create_leaf = NTreeC3.create_leaf #U32.t
+
+//noextract
+let pack_tree = NTreeC3.pack_tree #U32.t
+
+let member = P1.member #U32.t
+//inline_for_extraction
+//let append_left = append_left #U32.t
+//let append_right = append_right #U32.t
+//let height = height #U32.t
+
+//let rotate_left = rotate_left #U32.t
+//let rotate_right = rotate_right #U32.t
+//let rotate_right_left = rotate_right_left #U32.t
+//let rotate_left_right = rotate_left_right #U32.t
+//
+//let is_balanced = is_balanced #U32.t
+//let rebalance_avl = rebalance_avl #U32.t
+//let insert_avl = insert_avl #U32.t
+
+(*)
+let one ()
+  : Steel (ref nat)
+  (emp)
+  (fun r -> vptr r)
+  (requires fun _ -> True)
+  (ensures fun _ _ _ -> True)
+  =
+  let r = malloc 1 in
+  r*)
+
+(*)
+let rec free_wds #a (ptr: t a) : Steel unit
+  (linked_tree ptr)
+  //(fun _ -> admit(); sladmit (); emp)
+  (fun _ -> admit(); sladmit (); emp)
+  (requires fun _ -> True)
+  (ensures fun _ _ _ -> True)
+  =
+  sladmit ();
+  let n = NTreeC3.unpack_tree ptr in
+  //free_wds (get_left n);
+  //free_wds (get_right n);
+  //free (get_size n);
+  //write (get_size n) 0;
+  pack_tree ptr (get_left n) (get_right n) (get_size n);
+  free ptr;
+  ()
+  //free (get_data n)
+*)
+
+(*)
+let create_leaf ()
+  : Steel (t U32.t)
+  (emp)
+  (fun ptr -> linked_tree ptr)
+  (requires fun _ -> True)
+  (ensures fun _ ptr h1 -> Trees.Leaf? (v_linked_tree ptr h1))
+  =
+  intro_linked_tree_leaf ();
+  null_t
+*)
+
+(*)
+let rec leftmost_p' (#a: eqtype) (x: Trees.tree a) (d: a) : a
+  = match x with
+  | Trees.Leaf -> d
+  | Trees.Node x l _ _ ->
+      let v = leftmost_p' l d in
+      if v = d then x else v
+let leftmost_p = leftmost_p' #U32.t
+
+let rec leftmost (ptr: t U32.t) (d: U32.t) : Steel U32.t
+  (linked_tree ptr)
+  (fun _ -> linked_tree ptr)
+  (requires fun _ -> True)
+  (ensures fun h0 x h1 ->
+    v_linked_tree ptr h0 == v_linked_tree ptr h1 /\
+    x == leftmost_p (v_linked_tree ptr h0) d
+  )
+  =
+  if is_null_t ptr then (
+    elim_linked_tree_leaf ptr;
+    return d
+  ) else (
+    let n = unpack_tree ptr in
+    let v = leftmost (get_left n) d in
+    let vr = if v = d then (get_data n) else v in
+    pack_tree ptr (get_left n) (get_right n) (get_size n);
+    return vr
+  )
+*)
+
+let destruct_linked_tree_leaf (ptr: t U32.t) : Steel unit
+  (linked_tree ptr) (fun _ -> emp)
+  (requires fun _ -> is_null_t ptr)
+  (ensures fun _ _ _ -> True)
+  = sladmit ()
+
+//inline_for_extraction
+let rec destruct (ptr: t U32.t) : Steel unit
+  (linked_tree ptr) (fun _ -> emp)
+  (requires fun _ -> True)
+  (ensures fun _ _ _ -> True)
+  =
+  sladmit ()
+  (*)
+  if is_null_t ptr then (
+    destruct_linked_tree_leaf ptr
+  ) else (
+    let n = unpack_tree ptr in
+    destruct (get_left n);
+    destruct (get_right n);
+    free (get_size n);
+    free ptr
+  )*)
+
+let main ()
+  //: Steel (t U32.t)
+  : Steel U32.t
+  (emp)
+  //(fun ptr -> linked_tree ptr)
+  (fun _ -> emp)
+  (requires fun _ -> True)
+  (ensures fun _ _ _-> True)
+  =
+  let l = create_leaf () in
+  let r = create_leaf () in
+  let sr = malloc 1 in
+  let v = 1ul in
+  let n = mk_node v l r sr in
+  let ptr = malloc n in
+  pack_tree ptr l r sr;
+  //let ptr = append_left ptr 0ul in
+  //let vr = leftmost ptr 12ul in
+  let b = member ptr 0ul in
+  let vr = if b then 42ul else 11ul in
+  //ptr
+  destruct ptr;
+  vr
+
+(*)
+open FStar.HyperStack.ST
+open FStar.HyperStack
+let main (): Stack Int32.t (fun _ -> true) (fun _ _ _ -> true) =
+  push_frame ();
+  let r = one () in
+  let n = mk_node 1ul null_t null_t r in
+  pop_frame ();
+  0l
