NTreeC3.fsti
@@ -148,4 +148,9 @@ val unpack_tree (#a: Type0) (ptr: t a)
           //(v_linked_tree (get_left node) h1)
           //(v_linked_tree (get_right node) h1) /\
         (sel ptr h1) == node
-      ))
+      ))*)
+
+val create_leaf (#a: Type0) (_: unit) : Steel (t a)
+  emp (fun ptr -> linked_tree ptr)
+  (requires fun _ -> True)
+  (ensures fun _ ptr h1 -> Trees.Leaf? (v_linked_tree ptr h1))
